coq/set/Lang1/Substitution.v
@@ -1,0 +1,42 @@
+Require Import List.
+
+Require Import Utils.Composition.
+
+Require Import Core.Set.
+
+Require Import Lang1.Valid.
+Require Import Lang1.Syntax.
+Require Import Lang1.Semantics.
+Require Import Lang1.Environment.
+
+Local Lemma rewrite_ : forall (p p' q:set -> Prop),
+    (forall x, p x <-> p' x) -> 
+    ((forall x, p x) <-> (forall x, q x) ) ->
+    ((forall x, p' x) <-> (forall x, q x)).
+Proof.
+    intros p p' q H1 [H2 H3]. split; intros H4.
+    - apply H2. intros x. rewrite (H1 x). apply H4.
+    - intros x. rewrite <- (H1 x). apply H3. assumption.
+Qed.
+
+Lemma Substitution : forall (e:Env) (f:nat -> nat) (p:Formula), Valid f p -> 
+    eval e (fmap f p) <-> eval (e ; f) p.
+Proof.
+    intros e f p. revert p f e. induction p as [|n m|p1 IH1 p2 IH2|n p1 IH1];
+    intros f e V.
+    - simpl. split; auto.
+    - simpl. split; auto.
+    - simpl.  apply ValidImp in V. destruct V as [V1 V2].
+      rewrite IH1, IH2.
+        + split; auto.
+        + assumption.
+        + assumption.
+    - simpl. apply ValidAll in V. destruct V as [V1 V2].
+      apply rewrite_ with (fun x => eval ((bind e (f n) x) ; f) p1).
+        + intros x. rewrite IH1.
+            { split; auto. }
+            { assumption. }
+        +
+
+Show.
+
