lean/hhg/diff.lean
@@ -1,0 +1,6 @@
+lemma L0 : "x" ≠ "y" :=
+begin
+  from dec_trivial  -- remember this, do not use 'cases' tactic on string
+end
+
+
