lean/hhg/while/AExp.lean
@@ -1,0 +1,17 @@
+import Env
+
+-- Shallow embedding for arithmetic expressions
+def AExp : Type := Env → ℕ
+
+def bindVar (x : string) (n : AExp) (s:Env) : Env :=
+  λ v, if v = x then n s else s v
+
+def aNum (n : ℕ) : AExp := λ _, n
+def aVar (x : string) : AExp := λ s, s x
+def x : AExp := aVar "x"
+def y : AExp := aVar "y"
+def z : AExp := aVar "z"
+
+def aPlus  (m n : AExp) : AExp := λ s, m s + n s
+
+
