lean/hhg/while/BExp.lean
@@ -1,0 +1,4 @@
+import Env
+
+-- Shallow embedding for boolean expressions
+def BExp : Type := Env -> Prop
