lean/hhg/while/Env.lean
@@ -1,2 +1,7 @@
 def Env  : Type := string → ℕ
 
+def env : list (string × ℕ) → Env
+| []        := λ s, 0
+| ((v,n) :: xs) := λ s, if s = v then n else env xs s
+
+
