lean/hhg/clean.sh
@@ -1,7 +1,6 @@
 #!/bin/sh
 
-DIR=`pwd`
 HOME=/home/john/Prog/lean/hhg
 cd ${HOME}
+    ./while/clean.sh
     rm -f *.olean
-cd ${DIR}
