lean/hhg/while/clean.sh
@@ -1,0 +1,5 @@
+#!/bin/sh
+
+HOME=/home/john/Prog/lean/hhg/while
+cd ${HOME}
+    rm -f *.olean
